Moved loop sort to separate file

theories/examples/list_sort.v
@@ -36,17 +36,6 @@ Definition list_sort_service : val :=
     "xs" <- lmerge "cmp" !"ys" !"zs";;
     send "c" #().
 
-Definition loop_sort_service_go : val :=
-  rec: "go" "c" :=
-    if: recv "c" then list_sort_service "c";; "go" "c"
-    else if: recv "c" then
-      let: "d" := start_chan "go" in
-      send "c" "d";;
-      "go" "c"
-    else #().
-Definition loop_sort_service : val := λ: <>,
-  start_chan loop_sort_service_go.
-
 Definition list_sort_client : val := λ: "cmp" "xs",
   let: "c" := start_chan list_sort_service in
   send "c" "cmp";; send "c" "xs";;
@@ -153,38 +142,6 @@ Section list_sort.
     iSplit; first done. iFrame. iSplit; iPureIntro.
     - by apply (Sorted_list_merge _).
     - rewrite (merge_Permutation R). by f_equiv.
-  Qed.
-
-  Definition loop_sort_protocol_aux (rec : iProto Σ) : iProto Σ :=
-    ((sort_protocol <++> rec) <+> ((<?> c, MSG c {{ c ↣ rec @ N }}; rec) <+> END))%proto.
-
-  Instance loop_sort_protocol_aux_contractive : Contractive loop_sort_protocol_aux.
-  Proof.
-    intros n p p' Hp. rewrite /loop_sort_protocol_aux.
-    f_contractive; f_equiv=> //. apply iProto_message_ne=> c /=; by repeat f_equiv.
-  Qed.
-  Definition loop_sort_protocol : iProto Σ := fixpoint loop_sort_protocol_aux.
-  Lemma loop_sort_protocol_unfold :
-    loop_sort_protocol ≡ loop_sort_protocol_aux loop_sort_protocol.
-  Proof. apply (fixpoint_unfold loop_sort_protocol_aux). Qed.
-
-  Lemma loop_sort_service_go_spec c :
-    {{{ c ↣ iProto_dual loop_sort_protocol @ N }}}
-      loop_sort_service_go c
-    {{{ RET #(); c ↣ END @ N }}}.
-  Proof.
-    iIntros (Ψ) "Hc HΨ". iLöb as "IH" forall (c Ψ).
-    wp_rec. rewrite {2}loop_sort_protocol_unfold.
-    wp_apply (branch_spec with "Hc"); iIntros ([]) "/= Hc"; wp_if.
-    { wp_apply (list_sort_service_spec with "Hc"); iIntros "Hc".
-      by wp_apply ("IH" with "Hc"). }
-    wp_apply (branch_spec with "Hc"); iIntros ([]) "/= Hc"; wp_if.
-    - wp_apply (start_chan_proto_spec N loop_sort_protocol); iIntros (d) "Hd".
-      { wp_apply ("IH" with "Hd"); auto. }
-      wp_apply (send_proto_spec with "Hc"); simpl.
-      iExists d; iSplit; first done. iIntros "{$Hd} !> Hc".
-      by wp_apply ("IH" with "Hc").
-    - by iApply "HΨ".
   Qed.
 
   Lemma list_sort_client_spec {A} (I : A → val → iProp Σ) R
