theories/examples/loop_sort.v
@@ -1,0 +1,52 @@
+From stdpp Require Import sorting.
+From osiris.channel Require Import proto_channel.
+From iris.heap_lang Require Import proofmode notation.
+From osiris.utils Require Import list.
+From osiris.examples Require Import list_sort.
+
+Definition loop_sort_service : val :=
+  rec: "go" "c" :=
+    if: recv "c" then list_sort_service "c";; "go" "c"
+    else if: recv "c" then
+      let: "d" := start_chan "go" in
+      send "c" "d";;
+      "go" "c"
+    else #().
+
+Section loop_sort.
+  Context `{!heapG Σ, !proto_chanG Σ} (N : namespace).
+
+  
+  Definition loop_sort_protocol_aux (rec : iProto Σ) : iProto Σ :=
+    ((sort_protocol <++> rec) <+> ((<?> c, MSG c {{ c ↣ rec @ N }}; rec) <+> END))%proto.
+
+  Instance loop_sort_protocol_aux_contractive : Contractive loop_sort_protocol_aux.
+  Proof.
+    intros n p p' Hp. rewrite /loop_sort_protocol_aux.
+    f_contractive; f_equiv=> //. apply iProto_message_ne=> c /=; by repeat f_equiv.
+  Qed.
+  Definition loop_sort_protocol : iProto Σ := fixpoint loop_sort_protocol_aux.
+  Lemma loop_sort_protocol_unfold :
+    loop_sort_protocol ≡ loop_sort_protocol_aux loop_sort_protocol.
+  Proof. apply (fixpoint_unfold loop_sort_protocol_aux). Qed.
+
+  Lemma loop_sort_service_spec c :
+    {{{ c ↣ iProto_dual loop_sort_protocol @ N }}}
+      loop_sort_service c
+    {{{ RET #(); c ↣ END @ N }}}.
+  Proof.
+    iIntros (Ψ) "Hc HΨ". iLöb as "IH" forall (c Ψ).
+    wp_rec. rewrite {2}loop_sort_protocol_unfold.
+    wp_apply (branch_spec with "Hc"); iIntros ([]) "/= Hc"; wp_if.
+    { wp_apply (list_sort_service_spec with "Hc"); iIntros "Hc".
+      by wp_apply ("IH" with "Hc"). }
+    wp_apply (branch_spec with "Hc"); iIntros ([]) "/= Hc"; wp_if.
+    - wp_apply (start_chan_proto_spec N loop_sort_protocol); iIntros (d) "Hd".
+      { wp_apply ("IH" with "Hd"); auto. }
+      wp_apply (send_proto_spec with "Hc"); simpl.
+      iExists d; iSplit; first done. iIntros "{$Hd} !> Hc".
+      by wp_apply ("IH" with "Hc").
+    - by iApply "HΨ".
+  Qed.
+
+End loop_sort.
